Imperative.v
@@ -23,17 +23,17 @@ Proof.
   apply eq_id_dec.
 Qed.
 
-Local Hint Resolve eq_exp_dec. 
+Local Hint Resolve eq_exp_dec.
 Local Hint Resolve eq_id_dec.
-  
+
 Tactic Notation "exp_cases" tactic (first) ident (c) :=
- first; 
+ first;
  [Case_aux c "ENum" | Case_aux c "EId" | Case_aux c "EPlus" ].
 
 
 Inductive eval : exp -> state -> nat -> Prop:=
    | eval_const : forall n st, eval (ENum n) st n
-   | eval_var: forall x st u, 
+   | eval_var: forall x st u,
         st x = Some u ->
         eval (EId x) st u
    | eval_plus  : forall e1 e2 st u v z,
@@ -42,25 +42,25 @@ Inductive eval : exp -> state -> nat -> Prop:=
         z = u + v ->
         eval (EPlus e1 e2) st z.
 Tactic Notation "eval_cases" tactic (first) ident (c) :=
- first; 
+ first;
  [Case_aux c "eval_const" | Case_aux c "eval_var" | Case_aux c "eval_plus" ].
 
 
-Lemma eval_const_aux : forall st n u, 
+Lemma eval_const_aux : forall st n u,
   eval (ENum n) st u -> u = n.
 Proof.
   intros.
   inversion H.
   crush.
-Qed.  
+Qed.
 
 Lemma eval_var_aux : forall st x u,
-  eval (EId x) st u -> st x = Some u.                      
+  eval (EId x) st u -> st x = Some u.
 Proof.
   intros. inversion H. assumption.
 Qed.
 
-(* Eval is deterministic *) 
+(* Eval is deterministic *)
 Theorem eval_is_det: forall e st u v,
   eval e st u ->
   eval e st v ->
@@ -70,23 +70,23 @@ Proof.
   generalize dependent v.
 
   eval_cases (induction H) Case.
-     intros; inversion H0; crush.     
+     intros; inversion H0; crush.
      intros; inversion H0; crush.
      intros. inversion H2. crush.
 Qed.
 
 
 Inductive cmd : Type :=
-  | CStop : cmd 
-  | CSkip : cmd 
+  | CStop : cmd
+  | CSkip : cmd
   | CAss  : id  -> exp -> cmd
   | CSeq  : cmd -> cmd -> cmd
   | CIf   : exp -> cmd -> cmd -> cmd
   | CWhile: exp -> cmd -> cmd.
 
 Tactic Notation "cmd_cases" tactic(first) ident(c) :=
-  first; 
-  [ Case_aux c "STOP" | Case_aux c "SKIP" 
+  first;
+  [ Case_aux c "STOP" | Case_aux c "SKIP"
   | Case_aux c "::=" | Case_aux c ";;"
   | Case_aux c "IFB" | Case_aux c "WHILE" ].
 
@@ -101,35 +101,61 @@ Notation "'IFB' c1 'THEN' c2 'ELSE' c3 'FI'" :=
   (CIf c1 c2 c3) (at level 80, right associativity).
 
 Inductive config : Type :=
-   | Config 
-       ( c : cmd) 
+   | Config
+       ( c : cmd)
        ( st: state).
 Notation "'〈' c ',' st '〉'" := (Config c st) (at level 0).
 
 Reserved Notation "cfg '⇒' cfg'" (at level 40).
 
+Definition cmd_of cfg :=
+  match cfg with
+    | Config c _ => c
+  end.
+
+Definition state_of cfg :=
+  match cfg with
+    | Config _ m => m
+  end.
+
+Definition is_stop cfg := cmd_of cfg = STOP.
+Definition is_not_stop cfg := cmd_of cfg <> STOP.
+
+
+
+(* lifiting reasoning about STOP to configurations *)
+
+(*
+Definition is_stop_config  := is_stop
+
+
+Definition is_not_stop_config  := is_not_stop
+
+*)
+
+
 Inductive step : config -> config -> Prop :=
-  | step_skip : forall st, 
+  | step_skip : forall st,
       〈 SKIP, st 〉 ⇒ 〈 STOP, st 〉
   | step_assign: forall x e v st st',
-       eval e st v -> 
+       eval e st v ->
        st' = update_st st x v ->
       〈 x ::= e, st 〉 ⇒  〈 STOP, st'〉
   | step_seq1 : forall c1 c1' c2 st st',
-      〈 c1, st 〉⇒ 〈 c1', st' 〉-> 
+      〈 c1, st 〉⇒ 〈 c1', st' 〉->
       c1' <> STOP ->
       〈 c1 ;; c2, st 〉⇒ 〈 c1' ;; c2, st' 〉
   | step_seq2 : forall c1 c2 st st',
-      〈 c1, st 〉⇒ 〈 STOP, st' 〉-> 
+      〈 c1, st 〉⇒ 〈 STOP, st' 〉->
       〈 c1 ;; c2, st 〉⇒ 〈 c2, st' 〉
-  | step_if1 : forall e u c1 c2 st, 
+  | step_if1 : forall e u c1 c2 st,
        eval e st u -> u <> 0 ->
       〈 IFB e THEN c1 ELSE c2 FI, st 〉⇒〈 c1, st 〉
-  | step_if2 : forall e c1 c2 st, 
+  | step_if2 : forall e c1 c2 st,
        eval e st 0 ->
       〈 IFB e THEN c1 ELSE c2 FI, st 〉⇒〈 c2, st 〉
   | step_while : forall e c st,
-      〈 WHILE e DO c END, st 〉⇒ 
+      〈 WHILE e DO c END, st 〉⇒
           〈 IFB e THEN c;; WHILE e DO c END ELSE SKIP FI, st 〉
 where "cfg '⇒' cfg' " := (step cfg cfg').
 
@@ -137,7 +163,5 @@ where "cfg '⇒' cfg' " := (step cfg cfg').
 Lemma eq_cmd_dec: forall c1 c2: cmd, {c1 = c2} + { c1<>c2 }.
 Proof.
   decide equality.
-Qed.  
-Local Hint Resolve eq_cmd_dec.  
-
-
+Qed.
+Local Hint Resolve eq_cmd_dec.
